Added inductive types

Expression.thy
@@ -10,6 +10,8 @@ datatype expr =
 | Proj expr nat
 | Inj nat "type list" expr
 | Case expr "expr list"
+| Fold type expr
+| Unfold type expr
 | TyAbs expr
 | TyApp expr type
 
@@ -21,6 +23,8 @@ primrec incr\<^sub>t\<^sub>e :: "nat \<Rightarrow> expr \<Rightarrow> expr" wher
 | "incr\<^sub>t\<^sub>e x (Proj e l) = Proj (incr\<^sub>t\<^sub>e x e) l"
 | "incr\<^sub>t\<^sub>e x (Inj l ts e) = Inj l (map (incr\<^sub>t\<^sub>t x) ts) (incr\<^sub>t\<^sub>e x e)"
 | "incr\<^sub>t\<^sub>e x (Case e cs) = Case (incr\<^sub>t\<^sub>e x e) (map (incr\<^sub>t\<^sub>e x) cs)"
+| "incr\<^sub>t\<^sub>e x (Fold t e) = Fold (incr\<^sub>t\<^sub>t (Suc x) t) (incr\<^sub>t\<^sub>e x e)"
+| "incr\<^sub>t\<^sub>e x (Unfold t e) = Unfold (incr\<^sub>t\<^sub>t (Suc x) t) (incr\<^sub>t\<^sub>e x e)"
 | "incr\<^sub>t\<^sub>e x (TyAbs e) = TyAbs (incr\<^sub>t\<^sub>e (Suc x) e)"
 | "incr\<^sub>t\<^sub>e x (TyApp e t) = TyApp (incr\<^sub>t\<^sub>e x e) (incr\<^sub>t\<^sub>t x t)"
 
@@ -32,6 +36,8 @@ primrec subst\<^sub>t\<^sub>e :: "nat \<Rightarrow> type \<Rightarrow> expr \<Ri
 | "subst\<^sub>t\<^sub>e x t' (Proj e l) = Proj (subst\<^sub>t\<^sub>e x t' e) l"
 | "subst\<^sub>t\<^sub>e x t' (Inj l ts e) = Inj l (map (subst\<^sub>t\<^sub>t x t') ts) (subst\<^sub>t\<^sub>e x t' e)"
 | "subst\<^sub>t\<^sub>e x t' (Case e cs) = Case (subst\<^sub>t\<^sub>e x t' e) (map (subst\<^sub>t\<^sub>e x t') cs)"
+| "subst\<^sub>t\<^sub>e x t' (Fold t e) = Fold (subst\<^sub>t\<^sub>t (Suc x) (incr\<^sub>t\<^sub>t 0 t') t) (subst\<^sub>t\<^sub>e x t' e)"
+| "subst\<^sub>t\<^sub>e x t' (Unfold t e) = Unfold (subst\<^sub>t\<^sub>t (Suc x) (incr\<^sub>t\<^sub>t 0 t') t) (subst\<^sub>t\<^sub>e x t' e)"
 | "subst\<^sub>t\<^sub>e x t' (TyAbs e) = TyAbs (subst\<^sub>t\<^sub>e (Suc x) (incr\<^sub>t\<^sub>t 0 t') e)"
 | "subst\<^sub>t\<^sub>e x t' (TyApp e t) = TyApp (subst\<^sub>t\<^sub>e x t' e) (subst\<^sub>t\<^sub>t x t' t)"
 
@@ -43,6 +49,8 @@ primrec incr\<^sub>e\<^sub>e :: "nat \<Rightarrow> expr \<Rightarrow> expr" wher
 | "incr\<^sub>e\<^sub>e x (Proj e l) = Proj (incr\<^sub>e\<^sub>e x e) l"
 | "incr\<^sub>e\<^sub>e x (Inj l ts e) = Inj l ts (incr\<^sub>e\<^sub>e x e)"
 | "incr\<^sub>e\<^sub>e x (Case e cs) = Case (incr\<^sub>e\<^sub>e x e) (map (incr\<^sub>e\<^sub>e (Suc x)) cs)"
+| "incr\<^sub>e\<^sub>e x (Fold t e) = Fold t (incr\<^sub>e\<^sub>e x e)"
+| "incr\<^sub>e\<^sub>e x (Unfold t e) = Unfold t (incr\<^sub>e\<^sub>e x e)"
 | "incr\<^sub>e\<^sub>e x (TyAbs e) = TyAbs (incr\<^sub>e\<^sub>e x e)"
 | "incr\<^sub>e\<^sub>e x (TyApp e t) = TyApp (incr\<^sub>e\<^sub>e x e) t"
 
@@ -54,6 +62,8 @@ primrec subst\<^sub>e\<^sub>e :: "nat \<Rightarrow> expr \<Rightarrow> expr \<Ri
 | "subst\<^sub>e\<^sub>e x e' (Proj e l) = Proj (subst\<^sub>e\<^sub>e x e' e) l"
 | "subst\<^sub>e\<^sub>e x e' (Inj l ts e) = Inj l ts (subst\<^sub>e\<^sub>e x e' e)"
 | "subst\<^sub>e\<^sub>e x e' (Case e cs) = Case (subst\<^sub>e\<^sub>e x e' e) (map (subst\<^sub>e\<^sub>e (Suc x) (incr\<^sub>e\<^sub>e 0 e')) cs)"
+| "subst\<^sub>e\<^sub>e x e' (Fold t e) = Fold t (subst\<^sub>e\<^sub>e x e' e)"
+| "subst\<^sub>e\<^sub>e x e' (Unfold t e) = Unfold t (subst\<^sub>e\<^sub>e x e' e)"
 | "subst\<^sub>e\<^sub>e x e' (TyAbs e) = TyAbs (subst\<^sub>e\<^sub>e x (incr\<^sub>t\<^sub>e 0 e') e)"
 | "subst\<^sub>e\<^sub>e x e' (TyApp e t) = TyApp (subst\<^sub>e\<^sub>e x e' e) t"
 
@@ -66,6 +76,8 @@ primrec is_value :: "expr \<Rightarrow> bool"
 | "is_value (Proj e l) = False"
 | "is_value (Inj l ts e) = is_value e"
 | "is_value (Case e cs) = False"
+| "is_value (Fold t e) = is_value e"
+| "is_value (Unfold t e) = False"
 | "is_value (TyAbs e) = True"
 | "is_value (TyApp e t) = False"
 | "is_value_f [] = True"
